Reduce some cheats and encounter a problem
The problem is that state_rel used to assume that all of the code in
the final g1 is present from the start in the code table. This is not
accurate when Install is involved, since clos_call is a phase that
introduces new code table entries.

compiler/backend/proofs/clos_callProofScript.sml
@@ -269,7 +269,7 @@ val state_rel_def = Define`
     (s.max_app = t.max_app) ∧
     LIST_REL (OPTREL (v_rel g l)) s.globals t.globals ∧
     fmap_rel (ref_rel (v_rel g l)) s.refs t.refs ∧
-    s.code = FEMPTY ∧ code_includes (SND g) t.code`;
+    s.code = FEMPTY (* ∧ code_includes (SND g) t.code *)`;
 
 val state_rel_max_app = Q.store_thm("state_rel_max_app",
   `state_rel g l s t ⇒ s.max_app = t.max_app`,
@@ -1561,7 +1561,8 @@ val code_inv_def = Define `
     s_code = FEMPTY /\
     s_cc = state_cc compile_inc t_cc /\
     t_co = state_co compile_inc s_co /\
-    (∀k. let (cfg,exp,aux) = s_co k in
+    (!k n. k <= n ==> subg (FST (FST (s_co k))) (FST (FST (s_co n)))) /\
+    (∀k. let (cfg,exp,aux) = s_co (k:num) in
            DISJOINT (IMAGE SUC (set (code_locs [exp])))
              (set (MAP FST (SND (FST cfg)))) /\
            wfg (FST cfg) /\
@@ -1583,17 +1584,19 @@ val code_rel_state_rel_install = store_thm("code_rel_state_rel_install",
     DISJOINT (FDOM t.code) (set (MAP FST (SND progs))) ∧
     ALL_DISTINCT (MAP FST (SND progs)) /\
     t.compile cfg' progs = SOME (bytes,data,FST (shift_seq 1 t.compile_oracle 0)) /\
-    ?exp1 aux1 g5. progs = (exp1,aux1) /\
-    calls [exp'] (FST cfg) = ([exp1],g5) /\
-    state_rel g1 l1
-     (r with
-      <|compile_oracle := shift_seq 1 r.compile_oracle;
-        code := r.code |++ aux|>)
-     (t with
-      <|compile_oracle := shift_seq 1 t.compile_oracle;
-        code := t.code |++ aux1|>) ∧
-    code_inv (r.code |++ aux) r.compile (shift_seq 1 r.compile_oracle)
-      (t.code |++ aux1) t.compile (shift_seq 1 t.compile_oracle)``,
+    ?exp1 aux1 g5 exp5 aux5 other.
+      progs = (exp1,aux1) /\
+      calls [exp'] (FST cfg) = ([exp1],g5) /\
+      state_rel g1 l1
+       (r with
+        <|compile_oracle := shift_seq 1 r.compile_oracle;
+          code := r.code |++ aux|>)
+       (t with
+        <|compile_oracle := shift_seq 1 t.compile_oracle;
+          code := t.code |++ aux1|>) ∧
+      code_inv (r.code |++ aux) r.compile (shift_seq 1 r.compile_oracle)
+        (t.code |++ aux1) t.compile (shift_seq 1 t.compile_oracle) /\
+      r.compile_oracle 1 = ((g5,other),exp5,aux5)``,
   Cases_on `calls [exp'] (FST cfg)` \\ fs []
   \\ imp_res_tac calls_sing \\ rveq \\ fs []
   \\ PairCases_on `progs` \\ fs [] \\ strip_tac
@@ -2180,7 +2183,10 @@ val calls_correct = Q.store_thm("calls_correct",
     \\ qexists_tac `ck+ck'` \\ fs [AC ADD_COMM ADD_ASSOC]
     \\ fs [evaluate_def])
   (* Op *)
-  \\ conj_tac >- (
+  \\ conj_tac
+
+ >- (
+
     fs [evaluate_def,calls_def] \\ rw []
     \\ pairarg_tac \\ fs [] \\ rw []
     \\ fs [evaluate_def]
@@ -2282,15 +2288,18 @@ val calls_correct = Q.store_thm("calls_correct",
       \\ disch_then (qspec_then `ck'` mp_tac) \\ fs [] \\ strip_tac
       \\ qexists_tac `ck+ck'` \\ fs [] \\ rfs [])
     \\ simp [env_rel_def] \\ rveq \\ fs []
-    \\ conj_tac THEN1 (fs [code_inv_def]
-                       \\ rpt (first_x_assum (qspec_then `0` mp_tac)) \\ fs [])
-    \\ conj_tac THEN1 (fs [code_inv_def]
-                       \\ rpt (first_x_assum (qspec_then `0` mp_tac)) \\ fs [])
-    \\ conj_tac THEN1 fs [wfv_state_def]
-    \\ conj_tac THEN1 (fs [code_inv_def]
-                       \\ rpt (first_x_assum (qspec_then `0` mp_tac)) \\ fs [])
-    \\ conj_tac THEN1 (fs [code_inv_def]
-                       \\ rpt (first_x_assum (qspec_then `0` mp_tac)) \\ fs [])
+    \\ rpt (conj_tac THEN1
+              (fs [code_inv_def,wfv_state_def]
+               \\ rpt (first_x_assum (qspec_then `0` mp_tac)) \\ fs []))
+    \\ `subg g5 g1` by
+     (fs [code_inv_def]
+      \\ qpat_x_assum `includes_state g1 s'.compile_oracle` mp_tac
+      \\ simp [includes_state_def] \\ strip_tac
+      \\ qpat_x_assum `_ = (res,s')` assume_tac
+      \\ drule evaluate_code \\ rw [] \\ fs [shift_seq_def]
+      \\ rpt (first_x_assum (qspecl_then [`1`,`k+n+1`] mp_tac)) \\ fs [])
+    \\ fs []
+
     \\ cheat)
   (* Fn *)
   \\ conj_tac >- (
@@ -3154,7 +3163,9 @@ val calls_correct = Q.store_thm("calls_correct",
     \\ simp[] \\ fs[]
     \\ fs[LIST_REL_EL_EQN]
     \\ rfs[EL_TAKE])
+
   \\ (reverse(Cases_on`b`) \\ fs[] \\ rveq >- (
+
     rveq \\ drule (GEN_ALL calls_el_sing)
     \\ disch_then (qspec_then`i`mp_tac)
     \\ impl_tac >- fs[wfg_def,recclosure_wf_def]
@@ -3169,7 +3180,9 @@ val calls_correct = Q.store_thm("calls_correct",
       \\ conj_tac >- fs[SUBSET_DEF]
       \\ qhdtm_x_assum`env_rel`mp_tac
       \\ simp[EL_ZIP]
-      \\ metis_tac[state_rel_with_clock,code_includes_subg,state_rel_def])
+      \\ rw []
+      THEN1 metis_tac[state_rel_with_clock,code_includes_subg,state_rel_def]
+      \\ cheat)
     \\ strip_tac
     \\ imp_res_tac calls_length \\ fs[]
     \\ simp[EL_ZIP]
@@ -3198,8 +3211,9 @@ val calls_correct = Q.store_thm("calls_correct",
     \\ IF_CASES_TAC \\ fs[] )
   \\ simp[EVAL``(closSem$dec_clock _ _).code``]
   \\ qmatch_assum_abbrev_tac`subg gd g1`
+
   \\ `code_includes (SND gd) t0.code`
-  by ( metis_tac[code_includes_subg,state_rel_def] )
+  by cheat
   \\ pop_assum mp_tac
   \\ `ALOOKUP (SND gd) (2 * i + loc + 1) = SOME (EL i (ZIP (MAP FST fns1,es)))`
   by (
@@ -3538,8 +3552,8 @@ val compile_correct = Q.store_thm("compile_correct",
 
 val semantics_calls = Q.store_thm("semantics_calls",
   `semantics (ffi:'ffi ffi_state) max_app FEMPTY co cc x <> Fail ==>
-   compile T x = (y,g1,aux) /\ every_Fn_SOME x ∧ every_Fn_vs_NONE x /\
-   ALL_DISTINCT (code_locs x) /\ FST (FST (co 0)) = (g1,aux) /\
+   compile T x = (y,g0,aux) /\ every_Fn_SOME x ∧ every_Fn_vs_NONE x /\
+   ALL_DISTINCT (code_locs x) /\ FST (FST (co 0)) = (g0,aux) /\
    code_inv FEMPTY cc co (FEMPTY |++ aux) cc1 co1 ==>
    semantics (ffi:'ffi ffi_state) max_app (FEMPTY |++ aux) co1 cc1 y =
    semantics (ffi:'ffi ffi_state) max_app FEMPTY co cc x`,
@@ -3553,24 +3567,38 @@ val semantics_calls = Q.store_thm("semantics_calls",
   \\ rpt (disch_then drule) \\ fs [EVAL ``wfg (LN,[])``]
   \\ disch_then (qspecl_then [`[]`,
       `initial_state ffi max_app (FOLDL $|+ FEMPTY aux) co1 cc1 k`,
-      `set (code_locs x) DIFF domain g1`,
+      `UNIV DIFF domain (FST (FST (FST (s2.compile_oracle 0))))`,
       `FST (FST (s2.compile_oracle 0))`] mp_tac)
   \\ simp []
-  \\ `wfg (g1,aux)` by
+  \\ `wfg (g0,aux)` by
    (match_mp_tac calls_wfg
     \\ asm_exists_tac \\ fs []
     \\ EVAL_TAC \\ fs [])
   \\ impl_tac THEN1
-   (fs [subg_def] \\ rpt conj_tac
+   (rpt conj_tac
     \\ fs [env_rel_def,state_rel_def,initial_state_def,code_includes_def]
     THEN1 (fs [wfv_state_def,initial_state_def,FEVERY_DEF,code_inv_def])
-    \\ cheat
- (* \\ full_simp_tac std_ss [GSYM FUPDATE_LIST]
-    \\ rpt strip_tac
-    \\ match_mp_tac mem_to_flookup
-    \\ fs [ALOOKUP_MEM]
-    \\ match_mp_tac calls_ALL_DISTINCT
-    \\ asm_exists_tac \\ fs [] *))
+    THEN1
+     (drule evaluate_code \\ rw [] \\ fs []
+      \\ fs [code_inv_def,shift_seq_def]
+      \\ first_x_assum (qspecl_then [`0`,`n`] mp_tac) \\ fs [])
+    THEN1 (fs [SUBSET_DEF] \\ cheat) (* needs to be assumed *)
+    THEN1 (fs [IN_DISJOINT,IN_DIFF] \\ metis_tac [])
+    THEN1
+     (drule evaluate_code \\ rw [] \\ fs []
+      \\ fs [code_inv_def,shift_seq_def]
+      \\ rpt (first_x_assum (qspecl_then [`n`] mp_tac)) \\ fs []
+      \\ Cases_on `co n` \\ fs [] \\ PairCases_on `r` \\ fs [])
+    THEN1
+     (full_simp_tac std_ss [GSYM FUPDATE_LIST]
+      \\ rpt strip_tac
+      \\ match_mp_tac mem_to_flookup
+      \\ fs [ALOOKUP_MEM]
+      \\ `aux = SND (g0,aux)` by fs []
+      \\ pop_assum (fn th => once_rewrite_tac [th])
+      \\ match_mp_tac calls_ALL_DISTINCT
+      \\ asm_exists_tac \\ fs [])
+    \\ fs [includes_state_def] \\ qexists_tac `0` \\ fs [])
   \\ strip_tac
   \\ qmatch_asmsub_abbrev_tac `(y,[],s4)`
   \\ qexists_tac `ck` \\ fs []
